# Untitled


Nice. Here is a clean path and the correct final expression.

Start from

- Torque about G: (l/2) N cosθ = (m l^2/12) α, so N cosθ = (m l/6) α and α = (6 N cosθ)/(m l).

- Translational y-equation: N - mg = m ( (α l/2) cosθ - (ω^2 l/2) sinθ ).

Solve for N from the translational equation:

N = mg + (m l/2)( α cosθ - ω^2 sinθ ).

Plug into the torque relation:

α = (6/(m l)) cosθ [ mg + (m l/2)( α cosθ - ω^2 sinθ ) ].

Simplify:

α = 6 g cosθ + 3 α cos^2 θ - 3 ω^2 sinθ cosθ.

Bring the α terms together:

α [1 - 3 cos^2 θ] = 6 g cosθ - 3 ω^2 sinθ cosθ.

Therefore the angular acceleration is

$$

\boxed{ \alpha = \frac{6 g \cos\theta - 3 \omega^2 \sin\theta \cos\theta}{1 - 3 \cos^2\theta} }

= \frac{3 \cos\theta (2 g - \omega^2 \sin\theta)}{1 - 3 \cos^2\theta},

$$

where \(\omega = \dot\theta\).

And the normal force (optional) from the translational equation:

$$

N = mg + \frac{m l}{2} \left( \alpha \cos\theta - \omega^2 \sin\theta \right).

$$

Note: Your previous step had an incorrect factor inside the torque relation; the correct relation is (l/2) N cosθ = (m l^2/12) α.