# 8. Bending


## Axial Bar Deformation


![](excalidraw-2025-11-04-17.43.20.excalidraw.svg)
%%[ðŸ–‹ Edit in Excalidraw](excalidraw-2025-11-04-17.43.20.excalidraw.md)%%


In the situation where there is a fixture on either side of a 1D axial bar, you can replace the right-hand side with an unknown reaction force.

Then, using the [flexibility matrix](6.%20Strain.md#^flexibility-matrix), you can solve for the missing reaction by enforcing that the strain is zero.

The 2D version of the flexibility matrix is:

$$\begin{Bmatrix}
\sigma_{xx}\\[4pt]
\sigma_{yy}\\[4pt]
\sigma_{xy}
\end{Bmatrix}
=
\frac{E}{1 - \nu ^2}
\begin{bmatrix}
1 & \nu & 0\\
\nu & 1 & 0\\
0 & 0 & \frac{1 - \nu}{2}
\end{bmatrix}
\begin{Bmatrix}
\epsilon_{xx}\\[4pt]
\epsilon_{yy}\\[4pt]
\gamma_{xy}
\end{Bmatrix}$$

Because we are only interested in $\sigma_{xx}$, this gets reduced to:

$$\sigma_{xx} = \frac{E}{1-\nu ^2} (\epsilon_{xx}+\nu \epsilon_{yy})$$

Neglecting the poisson effect (because this is a 1D problem) makes $\nu \to 0$ and reduces the above equation:

$$\sigma_{xx} = E \cdot \epsilon_{xx}$$

---

An easier way to apply this in the above scenario is to solve for the strain, and then force it to be zero (or some other value.)

For discrete (1D/axial) forces,

$$\epsilon_{xx} = \frac{\sigma_{xx}}{E} = \frac{N}{EA}$$

where $N$ is the normal force, $E$ is Young's Modulus, and $A$ is cross-section area. 

More generally,

$$u(x_c)-u(0) = \int\limits ^{x_c}_0 \frac{N(x)}{E(x)A(x)}\,dx$$

---

![](excalidraw-2025-11-08-14.01.34.excalidraw.svg)
%%[ðŸ–‹ Edit in Excalidraw](excalidraw-2025-11-08-14.01.34.excalidraw.md)%%

There are two ways to solve for the normal force given a force per unit length like $p(x)$.

**Method 1**

Solve for the reaction force $R_x$ by solving:

$$\sum F_x = R_x + \int _0^L p(x) \, dx = 0$$

Then, at the cross section, you can find N with:

$$\sum F_x = R_x + \int _0^x p(x)\, dx + N(x)=0$$

Solving this gives you the desired function for $N(x)$.

**Method 2**

You can ignore the restraint and integrate from the other side. Skip to taking a cross section, then solve the equation:

$$\sum F_x = -N + \int _x ^L p(x)\,dx = 0$$



## Beam Bending


We want to find the displacement as a function of $x$, i.e. $y(x)$. The derivatives of this function are:

- $y'(x)$: **Slope** of bending
- $y''(x)$: **Curvature** of bending.


First, we calculate the [Bending Moment](Beams.md) $M(x)$. The *curvature* of bending can be found directly with this:

$$\text{Curvature}=y''(x) = \frac{M(x)}{EI}$$

where $I$ is the second moment of area and $E$ is the elasticity. 

From here, it is fairly simple to find the rest:

$$\text{Slope} = y'(x) = \int_0^x\frac{M(u)}{EI}\,du$$

and

$$
\text{Deformation} = y(x) = \int _0^x \int _0^{u_2}\frac{M(u_1)}{EI}\,du_1
$$

This assumes that $y_0=0$. If we don't want to enforce this constraint, the most general form is:

$$EI \frac{d^2y}{dx^2}=M(x)$$

or

$$
E I, y(x) = \int \left(\int M(x),dx\right) dx + C_1x + C_2  
$$

 