# 2. Equation of Hydrostatics



At rest, fluid has no shear stress:

$$T_{xy}=T_{xz}=T_{zx}=0$$

and 

$$T_{xx}=T_{yy}=T_{zz}=-p \quad \text{ (pressure)}$$


This idea that the pressure in all directions is the same is known as **Pascal's Law**. It holds so long that there is no shear stress. More specifically:

> A *change* in pressure at any point in an enclosed incompressible fluid at rest is transmitted equally and undiminished to all points in all directions throughout the fluid, and the force due to the pressure acts at right angles to the enclosing walls.

When gravity is involved, this is:

$$\Delta p = \rho g \Delta h$$

--- 

The equations of hydrostatics, in vector form, are:

$$
\rho \mathbf a = \rho \mathbf g - \nabla p
$$

Where $\mathbf a$ is the acceleration vector (field?), and $\mathbf g$ is the external force field. 

In the special case when $\mathbf a = \vec 0$, 

$$0 = \rho \mathbf g - \nabla p$$


If $\mathbf g$ is simply gravity, then:

$$\mathbf  g = -g \hat k$$


In this case, where gravity acts only in the $\hat z$ direction, the equations of hydrostatics reduce to:

$$
\begin{cases}
(x);\qquad 0 &= - \frac{\partial p}{\partial x} \\ 
(y); \qquad 0 &= - \frac{\partial p}{\partial y} \\
(z); \qquad 0 &= -\rho g- \frac{\partial p}{\partial z} \\
\end{cases}
$$

From this, we can see that pressure does not change in the x and z axes, when gravity acts in the z axis. To solve for pressure, we can isolate the equation:

$$0 = -\rho g- \frac{\partial p}{\partial z}$$

i.e.

$$- \gamma = \frac{\partial \rho}{\partial z}$$

### Incompressible Fluids

Solving this gives an expression for pressure gives:

$$p-p_0 = - \int \limits _{z_0}^{z_1} \rho g \; dz$$

where $p_0$ is the pressure at $z_0$. 

$\gamma = \rho g$  is the **specific weight**; i.e. weight per unit volume. In *incompressible fluids where $\rho$ is constant*, the specific weight is also constant. This simplifies the above equation for pressure into:

$$p = p_0 + \gamma (z_0 - z)$$
^hydrostatic-pressure
### Compressibile Fluids

We can solve $- \gamma = \frac{\partial \rho}{\partial z}$ for compressible fluids, but we must also consider the variation of $\rho$ in the integral. 

If the gas is idea, where $p = \rho R T$, we can substitute it into the equation above. First, rearranging the ideal gas law gives:

$$\rho = \frac{p}{RT}$$

Then substituting this in:

$$\frac{\partial p}{\partial z} = -\gamma = - p g = - \frac{\rho g}{RT}$$

Separation of variables gives:

$$\int _{p_1}^{p_2} \frac{\partial p}{p} = \frac{-g}{R} \int _{z_1}^{z_2}\frac{\partial z}{T}$$

Solving:

$$p_2 = p_1 \exp \left[ -\frac{g(z_2-z_1)}{RT_0}\right]$$
### Hydrostatic Force on a Planar Surface

Imagine that a slanted surface has a force acting on it. From the book, this is:

![[IMG_0412.jpeg]]


The force acting on $dA$ is:

$$dF = \gamma h \,dA$$

This is because pressure is given as $p = \cancelto {0}{p_0}+\gamma (z_0-z) = \gamma h$ , and force is pressure times area.  Integrating gives:

$$F_R = \iint_A \gamma h \, dA = \iint_A \gamma y \sin (\theta ) \, dA = \gamma \sin (\theta) \iint _Ay \, dA $$

The quantity $\iint _A y\,dA$ is the *first* moment of area, which is simply the centroid $y_c$ times the area: $\iint _A y\,dA = y_cA$ . This lets us say that the force on the surface is:

$$F_R= \gamma A y_c \sin (\theta) = \gamma h_c A$$

where $h_c$ is the vertical distance from the top of the fluid to the centroid of the surface. In other words, the force is the pressure at the centroid of the surface, times the area of that surface.

But it is important to note that the force *is not applied at the centroid.* Instead, the equivalent point of application can be derived with the following:

An equivalent point force must satisfy moment equilibrium:

$$\begin{aligned}
F_Ry_R &= \iint _A y \,dF \\
 &=\iint _A \gamma \sin(\theta) y^2  dA\\
\big[\gamma A y_c \sin (\theta)\big] y_R&= \gamma \sin(\theta) \iint _A y\, dA\\
y&_R=\frac{\iint _A y^2\, dA}{y_cA}
\end{aligned}
$$

Because $\iint_A y^2\,dA$ is the *second* moment of area, $I_x$, this can also be expressed as:

$$y_R= \frac{I_x}{y_cA}$$

Where the $x$-axis intersects the free surface (see figure above). If instead it is easier to use the moment of inertia where the reference axis passes through the centroid, the parallel axis theorem allows us to say:

$$y_R = \frac{I_{xc}}{y_cA}+y_c$$

where $I_{xc}$ is the second moment of area *through the centroid*.

A similar derivation can be applied for $x$:

$$x_R = \frac{\iint_A xy\,dA}{y_cA}$$

Again, using the parallel axis theorem will let us say:

$$x_R= \frac{I_{xyc}}{y_cA}+x_c$$

where $I_{xyc}$ is the product










--- 



